changed definition of CPL and K axioms; proved few more lemmas

globalCompletenessScript.sml
@@ -22,32 +22,40 @@ val (KGproof_rules, KGproof_ind, KGproof_cases) = Hol_reln`
 `;    
 *)
  
+ (*
+ TODO
+  10 Sep 
+
+  DONE 1. Change CPLAxioms to use ptaut; (ptaut includes all the propositional axioms)
+  {might use Logics of Time and Computation. R. I. Goldblatt CSLI Lecture Notes Number 7,
+Center for the Study of Language and Information, Stanford, 1987}
+
+  DONE 2. use subst instead of set comprehension (?) (use atomic formulae in the set)
+*)
 
 Definition CPLAxioms_def:
-CPLAxioms = {A -> (B -> A) | T } ∪ 
-            {NOT (NOT A) -> A | T} ∪
-            {(A -> (B ->C)) -> ((A -> B) -> (B -> C))| T} 
+CPLAxioms = {a | ptaut a}
 End
 
-
-(* add type constraint *)
 Definition KAxioms_def:
-  KAxioms = CPLAxioms ∪
-           {(□ (A -> B)) -> ((□ A) -> (□ B)) | T}
+  KAxioms = 
+      CPLAxioms 
+    ∪
+      {(□ (VAR 0 -> VAR 1)) -> ((□ (VAR 0)) -> (□ (VAR 1)))}
 End
 
-
-fs[]
-rw[]
-simp[]
-metis_tac[]
-(* how to make Ax into a parameter gtt takes rather than a universal variable *)
 Inductive gtt:
 	(∀f. f ∈ G ⇒ gtt Ax G f) ∧
-	(∀f. f ∈ Ax ∧ (Ax = CPLAxioms ∨ Ax = KAxioms) ⇒ gtt Ax G f) ∧
-	(∀f1 f2. gtt Ax G f1 ∧ gtt Ax G (IMP f1 f2) ⇒ gtt Ax G f2) ∧
+	(∀f s. f ∈ Ax ⇒ gtt Ax G (subst s f)) ∧ 
+	(∀f1 f2. gtt Ax G f1 ∧ gtt Ax G (f1 -> f2) ⇒ gtt Ax G f2) ∧
 	(∀f. gtt Ax G f ⇒ gtt Ax G (□ f))
 End
+
+Theorem subst_compose:
+  ∀f g x. subst g (subst f x) = subst ((subst g) o f) x 
+Proof
+  Induct_on `x` >> rw[subst_def]
+QED
 
 Theorem gttSubst:
  ∀s f. gtt Ax G f ⇒ gtt Ax {subst s g | g ∈ G} (subst s f)
@@ -56,25 +64,61 @@ Proof
   rw[gtt_rules, subst_def] 
     >- (`(subst s f) ∈ {subst s g| g ∈ G}` suffices_by rw[gtt_rules] 
           >> fs[] >> metis_tac[])
-    >- (`(subst s f) ∈ CPLAxioms` suffices_by rw[gtt_rules] 
-          >> fs[CPLAxioms_def] >> rw[subst_def] >> cheat >> cheat >> cheat)
-    >- (`(subst s f) ∈ KAxioms` suffices_by rw[gtt_rules] 
-          >> fs[KAxioms_def] >> rw[subst_def] >> cheat)
-
+    >- (rw[subst_compose] >> rw[gtt_rules])
+    >> `!s. (subst s (f -> f')) = ((subst s f) -> (subst s f'))` 
+          by metis_tac[subst_def,IMP_def] 
+          >> metis_tac[gtt_rules]
 QED
 
+Theorem gttEmpG:
+  ∀s f. gtt Ax ∅ f ⇒ gtt Ax ∅ (subst s f)
+Proof
+  Induct_on `gtt` >> 
+  rw[gtt_rules, subst_def] 
+    >- (rw[subst_compose] >> rw[gtt_rules])
+    >> `!s. (subst s (f -> f')) = ((subst s f) -> (subst s f'))` 
+          by metis_tac[subst_def,IMP_def] 
+          >> metis_tac[gtt_rules]
+QED
+
+Theorem subst_self:
+  ∀f. f = subst (λi. VAR i) f 
+Proof 
+  Induct_on `f` >> simp[subst_def]
+QED
+
+Theorem gttAx:
+  ∀f s. f ∈ Ax ⇒ gtt Ax G f 
+Proof
+  rw[] >> `∀s. gtt Ax G (subst s f)` by rw[gtt_rules]
+  >>  `f = subst (λi. VAR i) f` by rw[subst_self] 
+  >> `gtt Ax G f` by metis_tac[]
+QED
 
 Theorem gTk:
-  ∀(p :'a form list). (KGproof Ax p) ⇒ (∀f. (MEM f p)  ⇒ gtt (Ax ∪ KAxioms) ∅ f)
+ ∀(p :num form list). (KGproof Ax p) ⇒ (∀f. (MEM f p)  ⇒ gtt (Ax ∪ KAxioms) ∅ f)
 Proof
   Induct_on `KGproof` >> rw[]
   >- metis_tac[]
   >- metis_tac[gtt_rules]
   >- metis_tac[]
-  >- (first_x_assum drule >> )
-
+  >- metis_tac[gttEmpG] 
+  >- simp[]
+  >- rw[gtt_rules]
+  >- simp[]
+  >- (rw[KAxioms_def, gtt_rules, gttAx] >> cheat) (* K Axiom*)
+  >- simp[]
+  >- cheat (* Diamond and box *)
+  >- simp[]
+  >- cheat (*box and diamond*)
+  >- (rw[subst_self, subst_def, gtt_rules, KAxioms_def, CPLAxioms_def] >> cheat)
+ (* `gtt (Ax ∪ KAxioms) ∅ (subst s f)` suffices_by rw[subst_self]
+  simp[KAxioms_def, CPLAxioms_def, gtt_rules]*)
+  >- simp[]
+  >> rw[gttAx]
+  (*>- (first_x_assum drule >>  qmatch_abbrev_tac`gtt Ax G f ⇒ gtt Ax G (subst s f)` >> rw[gttSubst])
+*)
 QED
-
 
 
 Theorem kTg:
